holds_on_raw_data_item_fmap

src/cbor/CBOR.Spec.Raw.Base.fst
@@ -239,3 +239,48 @@ let raw_data_item_fmap_eq
     assert_norm (raw_data_item_fmap f (Array len v) == f (Array len (wf_list_map v (raw_data_item_fmap f))));
     wf_list_map_eq (raw_data_item_fmap f) v
   | _ -> ()
+
+#push-options "--z3rlimit 32"
+
+#restart-solver
+let rec holds_on_raw_data_item_fmap_gen
+  (f: raw_data_item -> raw_data_item)
+  (p q: raw_data_item -> bool)
+  (prf: (x: raw_data_item) -> Lemma
+    (requires (pre_holds_on_raw_data_item p x == true))
+    (ensures (holds_on_raw_data_item (p `andp` q) (f x) == true))
+  )
+  (x: raw_data_item)
+: Lemma
+  (requires (pre_holds_on_raw_data_item p x == true))
+  (ensures (holds_on_raw_data_item (p `andp` q) (raw_data_item_fmap f x) == true))
+= let x' = raw_data_item_fmap f x in
+  raw_data_item_fmap_eq f x;
+  match x with
+  | Tagged tag v ->
+    holds_on_raw_data_item_eq p v;
+    holds_on_raw_data_item_fmap_gen f p q prf v;
+    let x_ = Tagged tag (raw_data_item_fmap f v) in
+    pre_holds_on_raw_data_item_implies (p `andp` q) p (fun _ -> ()) x_;
+    prf x_
+  | Array len v ->
+    list_for_all_map (raw_data_item_fmap f) v (holds_on_raw_data_item p) (holds_on_raw_data_item (p `andp` q)) (fun x ->
+      holds_on_raw_data_item_eq p x;
+      holds_on_raw_data_item_fmap_gen f p q prf x
+    );
+    let x_ = Array len (List.Tot.map (raw_data_item_fmap f) v) in
+    pre_holds_on_raw_data_item_implies (p `andp` q) p (fun _ -> ()) x_;
+    prf x_
+  | Map len v ->
+    list_for_all_map (apply_on_pair (raw_data_item_fmap f)) v (holds_on_pair (holds_on_raw_data_item p)) (holds_on_pair (holds_on_raw_data_item (p `andp` q))) (fun x ->
+      holds_on_raw_data_item_eq p (fst x);
+      holds_on_raw_data_item_fmap_gen f p q prf (fst x);
+      holds_on_raw_data_item_eq p (snd x);
+      holds_on_raw_data_item_fmap_gen f p q prf (snd x)
+    );
+    let x_ = Map len (List.Tot.map (apply_on_pair (raw_data_item_fmap f)) v) in
+    pre_holds_on_raw_data_item_implies (p `andp` q) p (fun _ -> ()) x_;
+    prf x_
+  | _ -> prf x
+
+#pop-options
